

Derivation of Gradient Descent

we know that

(cost function) \rightarrow mean squared error

$$J(w, b) = \frac{1}{2m} \sum_{i=1}^m (f_{w,b}(x_i) - (y_i))^2$$

where $f_{w,b}(x) = wx + b$

$m \rightarrow$ no. of tuples

$$w = w - \alpha \frac{\partial J(w, b)}{\partial w}$$

$$b = b - \alpha \frac{\partial J(w, b)}{\partial b}$$

this process will be repeated upto the point of convergence

$$\begin{aligned}
 \frac{\partial}{\partial \omega} J(\omega, b) &= \frac{\partial}{\partial \omega} \frac{1}{2m} \sum_{i=1}^m \left(\omega x_i + b - y_i \right)^2 \\
 &= \frac{\partial}{\partial \omega} \frac{1}{2m} \sum_{i=1}^m (\omega x_i + b - y_i)^2 \\
 &= \frac{1}{m} \sum_{i=1}^m (\omega x_i + b - y_i) \cdot x_i \\
 &= \frac{1}{m} \sum_{i=1}^m (\omega x_i + b - y_i) \cdot x_i
 \end{aligned}$$

From chain rule,

$$\boxed{\frac{\partial}{\partial \omega} J(\omega, b) = \frac{1}{m} \sum_{i=1}^m (\omega x_i + b - y_i) \cdot x_i}$$

$$\begin{aligned}
 \frac{\partial}{\partial b} J(\omega, b) &= \frac{\partial}{\partial b} \sum_{i=1}^m (\omega x_i + b - y_i)^2 \times \frac{1}{2m} \\
 &= \frac{\partial}{\partial b} \sum_{i=1}^m (\omega x_i + b - y_i)^2 \times \frac{1}{2m} \\
 &= \frac{1}{2m} \sum_{i=1}^m (\omega x_i + b - y_i) \times \frac{\partial}{\partial b} (\omega x_i + b - y_i)
 \end{aligned}$$

$$\boxed{\frac{\partial}{\partial b} J(\omega, b) = \frac{1}{m} \sum_{i=1}^m (\omega x_i + b - y_i)}$$

$$\begin{aligned}
 \omega &= \omega - \alpha \left(\frac{\sum_{i=1}^m (\omega x_i + b - y_i) x_i}{m} \right) \\
 b &= b - \alpha \left(\frac{\sum_{i=1}^m (\omega x_i + b - y_i)}{m} \right)
 \end{aligned}$$

→ Gradient descent for linear Regression